\titre{}
\theme{derivation}
\auteur{Nathan Scheinmann}
\niveau{3M}
\source{musy}
\type{serie}
\piments{1}
\pts{}
\annee{2526}

\contenu{
\tcblower
Dériver les fonctions.
\begin{tasks}(2)
\task $f(x)=(1-x)^{20}$
\task $f(x)=\left(x^2+1\right)^4$
\task $f(x)=\left(x^2+1\right)^3\left(2-x^3\right)^2$
\task $f(x)=\left(7 x^2-\frac{4}{x}+6\right)^6$
\task $f(x)=\frac{1+\sqrt{x}}{1+\sqrt{2 x}}$
\task $f(x)=\frac{2}{\left(x^2-x+1\right)^2}$
\task $f(x)=\frac{1}{\sqrt{a^2-x^2}}$
\task $f(x)=\left(\frac{1+x}{1-x}\right)^2$
\task $f(x)=\frac{x^2}{\sqrt{x^2+a^2}}$
\end{tasks}
}
\correction{
\tcblower
{\scriptsize \textit{Correction générée par IA}}

\begin{tasks}(2)
\task $f'(x) = 20(1-x)^{19} \cdot (-1) = -20(1-x)^{19}$

\task $f'(x) = 4(x^2+1)^3 \cdot 2x = 8x(x^2+1)^3$

\task
\( \begin{aligned}
f'(x) &= 3(x^2+1)^2 \cdot 2x \cdot (2-x^3)^2 + (x^2+1)^3 \cdot 2(2-x^3) \cdot (-3x^2) \\
&= 6x(x^2+1)^2(2-x^3)^2 - 6x^2(x^2+1)^3(2-x^3)
\end{aligned} \)

\task $f'(x) = 6\left(7x^2-\dfrac{4}{x}+6\right)^5 \cdot \left(14x+\dfrac{4}{x^2}\right)$

\task
\( \begin{aligned}
f'(x) &= \dfrac{\dfrac{1}{2\sqrt{x}}(1+\sqrt{2x}) - (1+\sqrt{x}) \cdot \dfrac{1}{\sqrt{2x}}}{(1+\sqrt{2x})^2} \\
&= \dfrac{\dfrac{1+\sqrt{2x}}{2\sqrt{x}} - \dfrac{1+\sqrt{x}}{\sqrt{2x}}}{(1+\sqrt{2x})^2}
\end{aligned} \)

\task $f'(x) = -\dfrac{2 \cdot 2(x^2-x+1) \cdot (2x-1)}{(x^2-x+1)^4} = -\dfrac{4(2x-1)}{(x^2-x+1)^3}$

\task $f'(x) = -\dfrac{1}{2}(a^2-x^2)^{-\frac{3}{2}} \cdot (-2x) = \dfrac{x}{(a^2-x^2)\sqrt{a^2-x^2}}$

\task
\( \begin{aligned}
f'(x) &= 2\left(\dfrac{1+x}{1-x}\right) \cdot \dfrac{1 \cdot (1-x) - (1+x) \cdot (-1)}{(1-x)^2} \\
&= 2\left(\dfrac{1+x}{1-x}\right) \cdot \dfrac{1-x+1+x}{(1-x)^2} \\
&= 2\left(\dfrac{1+x}{1-x}\right) \cdot \dfrac{2}{(1-x)^2} \\
&= \dfrac{4(1+x)}{(1-x)^3}
\end{aligned} \)

\task
\( \begin{aligned}
f'(x) &= \dfrac{2x\sqrt{x^2+a^2} - x^2 \cdot \dfrac{2x}{2\sqrt{x^2+a^2}}}{x^2+a^2} \\
&= \dfrac{2x\sqrt{x^2+a^2} - \dfrac{x^3}{\sqrt{x^2+a^2}}}{x^2+a^2} \\
&= \dfrac{2x(x^2+a^2) - x^3}{(x^2+a^2)\sqrt{x^2+a^2}} \\
&= \dfrac{2x^3 + 2a^2x - x^3}{(x^2+a^2)^{\frac{3}{2}}} \\
&= \dfrac{x^3 + 2a^2x}{(x^2+a^2)\sqrt{x^2+a^2}}
\end{aligned} \)
\end{tasks}
}

