\titre{}
\theme{derivation}
\auteur{Nathan Scheinmann}
\niveau{3M}
\source{sesamath3e}
\type{serie}
\piments{2}
\pts{}
\annee{2425}

\contenu{
	{\bfseries Entraînement individuel}
\tcblower
Utiliser les formules de dérivation pour  déterminer (donner des réponses sans exposant négatif ou fractionnaire) :
\begin{tasks}(3)
\task $\displaystyle \left(\dfrac{4}{x}\right)'$
\task $\displaystyle \left(\dfrac{-18}{x}\right)'$
\task $\displaystyle \left(\dfrac{1}{x^{2}}\right)'$
\task $\displaystyle \left(\dfrac{1}{3x^{3}}\right)'$
\task $\displaystyle \left(\dfrac{24}{x^{2}}\right)'$
\task $\displaystyle \left(\dfrac{1}{\sqrt{x}}\right)'$
\task $\displaystyle \left(\dfrac{1}{x\sqrt{x}}\right)'$
\task $\displaystyle \left(x^{2}-\dfrac{1}{2x}\right)'$
\task $\displaystyle \left(\dfrac{x^{2}}{x^{3}+1}\right)'$
\task $\displaystyle \left(\dfrac{1+2u^{3}}{2u}\right)'$
\task $\displaystyle ((2x+3)(3x-7))'$
\task $\displaystyle \bigl(x^{2}(1+\sqrt{x})\bigr)'$
\task $\displaystyle ((x^{3}-x)(x^{2}-9))'$
\task $\displaystyle \left(\dfrac{x^{2}+1}{4x}\right)'$
\end{tasks}
}
\correction{
\tcblower

\begin{tasks}(2)
\task $-\dfrac{4}{x^2}$

\task $\dfrac{18}{x^2}$

\task $-\dfrac{2}{x^3}$

\task $-\dfrac{1}{x^4}$

\task $-\dfrac{48}{x^3}$

\task $-\dfrac{1}{2x^{\frac{3}{2}}} = -\dfrac{1}{2x\sqrt{x}}$

\task $-\dfrac{3}{2x^{\frac{5}{2}}} = -\dfrac{3}{2x^2\sqrt{x}}$

\task $2x + \dfrac{1}{2x^2}$

\task* $\dfrac{2x(x^3+1) - x^2 \cdot 3x^2}{(x^3+1)^2} = \dfrac{2x^4 + 2x - 3x^4}{(x^3+1)^2} = \dfrac{-x^4 + 2x}{(x^3+1)^2}$

\task* $\dfrac{6u^2 \cdot 2u - (1+2u^3) \cdot 2}{4u^2} = \dfrac{12u^3 - 2 - 4u^3}{4u^2} = \dfrac{8u^3 - 2}{4u^2} = \dfrac{4u^3 - 1}{2u^2}$

\task* $(2)(3x-7) + (2x+3)(3) = 6x - 14 + 6x + 9 = 12x - 5$

\task* $2x(1+\sqrt{x}) + x^2 \cdot \dfrac{1}{2\sqrt{x}} = 2x + 2x\sqrt{x} + \dfrac{x^2}{2\sqrt{x}} = 2x + 2x\sqrt{x} + \dfrac{x\sqrt{x}}{2}$

\task* $(3x^2-1)(x^2-9) + (x^3-x)(2x) = 3x^4 - 27x^2 - x^2 + 9 + 2x^4 - 2x^2 = 5x^4 - 30x^2 + 9$

\task* $\dfrac{2x \cdot 4x - (x^2+1) \cdot 4}{16x^2} = \dfrac{8x^2 - 4x^2 - 4}{16x^2} = \dfrac{4x^2 - 4}{16x^2} = \dfrac{x^2 - 1}{4x^2}$
\end{tasks}
}

