\titre{}
\theme{derivation}
\auteur{Nathan Scheinmann}
\niveau{3M}
\source{sesamath3e}
\type{serie}
\piments{2}
\pts{}
\annee{2425}

\contenu{
\tcblower
Déterminer l’équation de la tangente à \(f:x\mapsto\dfrac{1}{x^2}\) au point \(\left(2\,;\,\dfrac{1}{4}\right)\).
}
\correction{
\tcblower

On a $f(x)=\dfrac{1}{x^2}=x^{-2}$, donc $f'(x)=-2x^{-3}=-\dfrac{2}{x^3}$.

Pour $x=2$, on a :
\begin{itemize}
\item $f(2)=\dfrac{1}{4}$
\item $f'(2)=-\dfrac{2}{8}=-\dfrac{1}{4}$
\end{itemize}

L'équation de la tangente est de la forme $y=f'(a)(x-a)+f(a)$, donc :

\( \begin{aligned}
y &= -\dfrac{1}{4}(x-2)+\dfrac{1}{4} \\
&= -\dfrac{1}{4}x+\dfrac{1}{2}+\dfrac{1}{4} \\
&= -\dfrac{1}{4}x+\dfrac{3}{4}
\end{aligned} \)

La tangente a pour équation $y=-\dfrac{1}{4}x+\dfrac{3}{4}$.
}

