\titre{}
\theme{derivation}
\auteur{Nathan Scheinmann}
\niveau{3M}
\source{sesamath3e}
\type{serie}
\piments{2}
\pts{}
\annee{2425}

\contenu{
\tcblower
Déterminer les dérivées des fonctions $f$ suivantes :
\begin{tasks}(2)
\task $f(x) = \sin(x) + 2\cos(x)$
\task $f(x) = \sin(x)\cos(x)$
\task $f(x) = (\sin(x) + 2\cos(x))\cos(x)$
\task $f(x) = \dfrac{\sin(x) + 1}{\sin(x) - 1}$
\task $f(x) = \dfrac{\cos(x) + 2}{\cos(x) + 3}$
\task $f(x) = \dfrac{\sin(3x)}{\cos(5x)}$
\task $f(x) = 2\cos(x) - \cos(2x)$
\task $f(x) = 2\sin^2(x) + 5\sin(x) - 3$
\task $f(x) = 3\sin^4(x) + \cos^3(x) - 1$
\task $f(x) = \dfrac{\sin(x)}{\sin(x) + \cos(x)}$
\task $f(x) = \dfrac{\sin(x)}{\cos(2x)}$
\task $f(x) = \sqrt{\cos(2x)} + 3\sin^2(x)$
\task $f(x) = x - \sin(x)\cos(x)$
\task $f(x) = \cos(x)(\sin^2(x) + 2)$
\task $f(x) = \dfrac{\sin(x) - x\cos(x)}{x\sin(x) + \cos(x)}$
\task $f(x) = \dfrac{x\sin(x) + \cos(x)}{\sin(x) - x\cos(x)}$
\task $f(x) = 2x\cos(x) + (x^2 - 2)\sin(x)$
\end{tasks}
}
\correction{
\tcblower
\textit{Generated by AI}

\begin{tasks}(2)
\task $f'(x) = \cos(x) - 2\sin(x)$

\task $f'(x) = \cos(x)\cos(x) + \sin(x)(-\sin(x)) = \cos^2(x) - \sin^2(x)$

\task $f'(x) = (\cos(x) - 2\sin(x))\cos(x) + (\sin(x) + 2\cos(x))(-\sin(x)) = \cos^2(x) - 2\sin(x)\cos(x) - \sin^2(x) - 2\sin(x)\cos(x) = \cos^2(x) - \sin^2(x) - 4\sin(x)\cos(x)$

\task $f'(x) = \dfrac{\cos(x)(\sin(x) - 1) - (\sin(x) + 1)\cos(x)}{(\sin(x) - 1)^2} = \dfrac{-2\cos(x)}{(\sin(x) - 1)^2}$

\task $f'(x) = \dfrac{-\sin(x)(\cos(x) + 3) - (\cos(x) + 2)(-\sin(x))}{(\cos(x) + 3)^2} = \dfrac{\sin(x)}{(\cos(x) + 3)^2}$

\task $f'(x) = \dfrac{3\cos(3x)\cos(5x) - \sin(3x)(-5\sin(5x))}{\cos^2(5x)} = \dfrac{3\cos(3x)\cos(5x) + 5\sin(3x)\sin(5x)}{\cos^2(5x)}$

\task $f'(x) = -2\sin(x) + 2\sin(2x)$

\task $f'(x) = 2 \cdot 2\sin(x)\cos(x) + 5\cos(x) = 4\sin(x)\cos(x) + 5\cos(x)$

\task $f'(x) = 3 \cdot 4\sin^3(x)\cos(x) + 3\cos^2(x)(-\sin(x)) = 12\sin^3(x)\cos(x) - 3\sin(x)\cos^2(x)$

\task $f'(x) = \dfrac{\cos(x)(\sin(x) + \cos(x)) - \sin(x)(\cos(x) - \sin(x))}{(\sin(x) + \cos(x))^2} = \dfrac{\cos^2(x) + \sin^2(x)}{(\sin(x) + \cos(x))^2} = \dfrac{1}{(\sin(x) + \cos(x))^2}$

\task $f'(x) = \dfrac{\cos(x)\cos(2x) - \sin(x)(-2\sin(2x))}{\cos^2(2x)} = \dfrac{\cos(x)\cos(2x) + 2\sin(x)\sin(2x)}{\cos^2(2x)}$

\task $f'(x) = \dfrac{-2\sin(2x)}{2\sqrt{\cos(2x)}} + 6\sin(x)\cos(x) = \dfrac{-\sin(2x)}{\sqrt{\cos(2x)}} + 6\sin(x)\cos(x)$

\task $f'(x) = 1 - (\cos(x)\cos(x) + \sin(x)(-\sin(x))) = 1 - \cos^2(x) + \sin^2(x)$

\task $f'(x) = -\sin(x)(\sin^2(x) + 2) + \cos(x)(2\sin(x)\cos(x)) = -\sin^3(x) - 2\sin(x) + 2\sin(x)\cos^2(x)$

\task $f'(x) = \dfrac{(\cos(x) - \cos(x) + x\sin(x))(x\sin(x) + \cos(x)) - (\sin(x) - x\cos(x))(\sin(x) + x\cos(x) - \sin(x))}{(x\sin(x) + \cos(x))^2} = \dfrac{x\sin(x)(x\sin(x) + \cos(x)) - (\sin(x) - x\cos(x))(x\cos(x))}{(x\sin(x) + \cos(x))^2}$

Simplification : $f'(x) = \dfrac{x^2\sin^2(x) + x\sin(x)\cos(x) - x\sin(x)\cos(x) + x^2\cos^2(x)}{(x\sin(x) + \cos(x))^2} = \dfrac{x^2}{(x\sin(x) + \cos(x))^2}$

\task $f'(x) = \dfrac{(\sin(x) + x\cos(x) - \sin(x))(\sin(x) - x\cos(x)) - (x\sin(x) + \cos(x))(\cos(x) - \cos(x) + x\sin(x))}{(\sin(x) - x\cos(x))^2}$

Simplification : $f'(x) = \dfrac{x\cos(x)(\sin(x) - x\cos(x)) - (x\sin(x) + \cos(x))(x\sin(x))}{(\sin(x) - x\cos(x))^2} = \dfrac{-x^2}{(\sin(x) - x\cos(x))^2}$

\task $f'(x) = 2\cos(x) - 2x\sin(x) + 2x\sin(x) + (x^2 - 2)\cos(x) = 2\cos(x) + (x^2 - 2)\cos(x) = x^2\cos(x)$
\end{tasks}
}

