\titre{}
\theme{limites}
\auteur{Nathan Scheinmann}
\niveau{3M}
\source{sesamath3e}
\type{serie}
\piments{4}
\pts{}
\annee{2425}

\contenu{
\tcblower
Calculer les limites suivantes.
\begin{tasks}(3)
\task $\displaystyle\lim_{x\to 3^+}\dfrac{\sqrt{x^2 - 4x + 3}}{x - 3}$
\task $\displaystyle\lim_{x\to 1}\dfrac{\sqrt{x^2 + x} - \sqrt{2}}{x - 1}$
\task $\displaystyle\lim_{x\to 1}\dfrac{\sqrt{x + 3} - \sqrt{3x + 1}}{x - 1}$
\task $\displaystyle\lim_{x\to 0^+}\dfrac{x}{\sqrt{1 + x^2} - 1}$
\task $\lim_{x \to -2^-} \dfrac{x + \sqrt{2 - x}}{x + 2}$
\end{tasks}
}
\correction{
	\tcblower

	\begin{tasks}(2)
\task Type «$ \dfrac{0}{0} $» :  

\(
\begin{aligned}
&\lim_{x \to 3^+} \dfrac{\sqrt{x^2 - 4x + 3}}{x - 3}\\
&= \lim_{x \to 3^+} \dfrac{\sqrt{(x - 1)(x - 3)}}{x - 3} \\
&= \lim_{x \to 3^+} \dfrac{\sqrt{x - 1} \cdot \sqrt{x - 3}}{x - 3} \\
&\stackrel{x \ne 3}{=} \lim_{x \to 3^+} \dfrac{\sqrt{x - 1}}{\sqrt{x - 3}^2} \cdot \sqrt{x - 3} \\
&= \lim_{x\to 3^+} \dfrac{\sqrt{x-1}}{\sqrt{x-3}}\\
&= +\infty
\end{aligned}
\)

\task Type «$ \dfrac{0}{0} $» :  

\(
\begin{aligned}
&\lim_{x \to 1} \dfrac{\sqrt{x^2 + x} - \sqrt{2}}{x - 1}\\
&= \lim_{x \to 1} \dfrac{x^2 + x - 2}{(x - 1)(\sqrt{x^2 + x} + \sqrt{2})} \\
&= \lim_{x \to 1} \dfrac{(x - 1)(x + 2)}{(x - 1)(\sqrt{x^2 + x} + \sqrt{2})} \\
&\stackrel{x \ne 1}{=} \lim_{x \to 1} \dfrac{x + 2}{\sqrt{x^2 + x} + \sqrt{2}} \\
&= \dfrac{3}{2\sqrt{2}}=\dfrac{3\sqrt{2}}{4}
\end{aligned}
\)

\task Type «$ \dfrac{0}{0} $» :  

\(
\begin{aligned}
&\lim_{x \to 1} \dfrac{\sqrt{x + 3} - \sqrt{3x + 1}}{x - 1}\\
&= \lim_{x \to 1} \dfrac{(x + 3) - (3x + 1)}{(x - 1)(\sqrt{x + 3} + \sqrt{3x + 1})} \\
&= \lim_{x \to 1} \dfrac{-2(x - 1)}{(x - 1)(\sqrt{x + 3} + \sqrt{3x + 1})} \\
&\stackrel{x \ne 1}{=} \lim_{x \to 1} \dfrac{-2}{\sqrt{x + 3} + \sqrt{3x + 1}}\\
&= \dfrac{-2}{4} = -\dfrac{1}{2}
\end{aligned}
\)

\task Type «$ \dfrac{0}{0} $» :  

\(
\begin{aligned}
&\lim_{x \to 0^+} \dfrac{x}{\sqrt{1 + x^2} - 1}\\
&= \lim_{x \to 0^+} \dfrac{x(\sqrt{1 + x^2} + 1)}{1 + x^2 - 1} \\
&= \lim_{x \to 0^+} \dfrac{x(\sqrt{1 + x^2} + 1)}{x^2} \\
&= \lim_{x \to 0^+} \dfrac{\sqrt{1 + x^2} + 1}{x}\\
&=+\infty
\end{aligned}
\)
\task Type «$ \dfrac{0}{0} $» :  

\(
\begin{aligned}
&\lim_{x \to -2^-} \dfrac{x + \sqrt{2 - x}}{x + 2}\\
&= \lim_{x\to -2^-} \dfrac{x + \sqrt{2 - x}}{x + 2} \cdot \dfrac{x - \sqrt{2 - x}}{x - \sqrt{2 - x}} \\
&= \lim_{x\to-2^-} \dfrac{x^2 - (2 - x)}{(x + 2)(x - \sqrt{2 - x})} \\
&= \lim_{x\to-2^-}\dfrac{x^2 + x - 2}{(x + 2)(x - \sqrt{2 - x})} \\
&= \lim_{x\to-2^-}\dfrac{(x + 2)(x - 1)}{(x + 2)(x - \sqrt{2 - x})} \\
&\stackrel{x \ne -2}{=} \lim_{x\to-2^-} \dfrac{x - 1}{x - \sqrt{2 - x}} \\
&= \dfrac{-3}{-2 - 2} = \dfrac{3}{4}
\end{aligned}
\)
\end{tasks}

}

